
\subsection{Exact equations of motion for spin-1}

\beq
\mathcal{L} 
	=	-\frac{1}{2} (D^\mu W^\nu - D^\nu W^\mu)^\dagger (D_\mu W_\nu - D_\nu W_\mu)
		+ m^2 W^{\mu \dagger} W_\mu - i \lambda e  W^{\mu \dagger} W^\nu F_{\mu\nu}
\eeq

where as usual $D$ is the long derivative $D^\mu = \partial^\mu + ieA^\mu$.

Obtain the equations of motion from the Euler-Lagrange equations:
\[
	\pd{\mathcal{L}}{W^{\dagger \alpha}} - \partial_\mu \pd{ \mathcal{L} }{ [\partial_\mu W^{\dagger \alpha}] } = 0
\]
Or equivalently, %TODO show this explicitly?
\[
	\pd{\mathcal{L}}{W^{\dagger \alpha}} - D_\mu \pd{ \mathcal{L} }{ [D_\mu W^{\dagger \alpha}] } = 0
\]

\beqa
\pd{\mathcal{L}}{W^{\dagger \alpha}} 
	&=&	\pd{}{W^{\dagger \alpha} } \left( m^2 W^{\mu \dagger} W_\mu - i \lambda e  W^{\mu \dagger} W^\nu F_{\mu\nu} \right )	\\
	&=&	m^2 W_\alpha - i e \lambda W^\nu F_{\alpha \nu} 	\\
\eeqa


\beqa
\pd{ \mathcal{L} }{ [D_\gamma W^{\dagger \alpha}] }
	&=& -\frac{1}{2} \pd{}{ [D_\gamma W^{\dagger \alpha}] }	 (D^\mu W^\nu - D^\nu W^\mu)^\dagger (D_\mu W_\nu - D_\nu W_\mu) 	\\
	&=& -\frac{1}{2} ( g^{\mu \gamma} g^\nu_\alpha - g^{\nu\gamma} g^\mu_\alpha)(D_\mu W_\nu - D_\nu W_\mu)	\\
	&=&  D_\alpha W^\gamma - D^\gamma W_\alpha \\
\eeqa


So the complete equation from Euler-Lagrange is
\beq \label{eq:ELeq}
		m^2 W_\alpha - i e \lambda W^\nu F_{\alpha \nu} + D_\mu (D^\mu W_\alpha - D_\alpha W^\mu) = 0
\eeq

This is a set of four coupled second order equations for the field $W$.  We rewrite as a set of first order equations by introducing a field $W_{\mu\nu} = D_\mu W_\nu - D_\nu W_\mu$.  So \eqref{eq:ELeq} becomes 
\beq
	m^2 W_\alpha - i e \lambda W^\mu F_{\alpha \mu} + D^\mu W_{\mu\alpha} = 0
\eeq

%TODO add note about two three-vectors to form a bispinor with?
$W^{\mu\nu}$ is antisymmetric and so has six degrees of freedom, corresponding to six independent fields.  Together with $W^\mu$ this represents a total of ten fields.  However, upon examination only some of these fields are dynamic.  The  fields $W^{0i}$ and $W^{i}$ appear in the equations with time derivatives, while the fields $W^{ij}$ and $W^0$ never do.  So it is only necessary to consider the former six fields.  So that these six fields all have the same dimension, we will define $\frac{W^{i0}}{m} = i \eta^i$.

We will now eliminate the extraneous fields and solve for $iD_0 W^i$, $iD_0 \eta^i$.

%%%%%%%%%%%%%%%%%%%%%%%%%%%%%%%%%%%%%%%%%%%%%%

\beq 
	m^2 W_\alpha - ie \lambda W^\nu F_{\alpha \nu} + D_\mu (D^\mu W_\alpha - D_\alpha W^\mu) = 0 
\eeq

Define $W_{\mu\nu} = D_\mu W_\nu - D_\nu W_\mu$.  
Then
\beq \label{eq:s1:EL1st}
	m^2 W_\alpha - ie \lambda W^\nu F_{\alpha \nu} + D^\mu W_{\mu \alpha} = 0
\eeq
To get the exact Hamiltonian of a bispinor, we can eliminate nondynamic fields.  

First consider \eqref{eq:s1:EL1st} with $\alpha=0$.
\beq
	m^2 W_0 - i e \lambda W^\nu F_{0\nu} + D^\mu W_{\mu0}
\eeq
\beq
	m^2 W_0 - i e \lambda W^j F_{0j} + D^j W_{j0}
\eeq

Solve this for $W_0$
\beq \label{eq:s1:w0}
	W_0 = \frac{1}{m^2} \left( i e \lambda W^j F_{0j} - D^j W_{j0} \right )
\eeq

Now, consider \eqref{eq:s1:EL1st} with $\alpha=i$
\beq
	m^2 W_i - ie \lambda W^\mu F_{i \mu} + D^\mu W_{\mu i} = 0
\eeq

\beq
	m^2 W_i - ie \lambda W^0 F_{i 0} + D^0 W_{0 i} - ie \lambda W^j F_{i j} + D^j W_{j i}= 0
\eeq

Using \eqref{eq:s1:w0} we can replace $W_0$

\beq
	m^2 W_i - \frac{i e \lambda}{m^2} \left( i e \lambda W^\nu F_{0\nu} - D^j W_{j0} \right ) F_{i 0} + D^0 W_{0 i} - ie \lambda W^j F_{i j} + D^j W_{j i}= 0
\eeq
Using $W_{ji} = D_j W_i - D_i W_j$
\beq
	m^2 W_i - \frac{i e \lambda}{m^2} \left( i e \lambda W^\nu F_{0\nu} - D^j W_{j0} \right ) F_{i 0} + D^0 W_{0 i} 
	- ie \lambda W^j F_{i j} + D^j (  D_j W_i - D_i W_j ) = 0
\eeq



Solve this for $D^0 W_{0i}$:

\beq \label{eq:s1:w0i}
	D^0 W_{0i} = - m^2 W_i  + \frac{i e \lambda}{m^2} \left( i e \lambda W^\nu F_{0\nu} - D^j W_{j0} \right ) F_{i 0} 
	+ ie \lambda W^j F_{i j} - D^j (  D_j W_i - D_i W_j )
\eeq


To get a similar equation for $W_i$, consider
\beq
	W_{i0} = D_i W_0 - D_0 W_i
\eeq
Then
\beq
	D^0 W_i = D_i W_0 - W_{i0}
\eeq
\beq \label{eq:s1:wi}
	D^0 W_i = D_i \frac{1}{m^2}\left( i e \lambda W^j F_{0j} - D^j W_{j0} \right )  - W_{i0}
\eeq

We now have equations that tell us the time evolution of a total of six fields: $W_i$ and $W_{i0}$.  We want to treat these as the components of some sort of bispinor.  To that end, first define $\eta_i = -i/m W_{i0}$ so that we have a pair of fields with the same mass dimension and hermiticity.  (Since $W_{i0} = D_i W_0 - D_0 W_i$ would pick up another minus sign under complex conjugation compared to $W_i$.)  Going the other way $W_{i0} = im \eta_i$.

Since eventually we want a nonrelativistic expression, we should write the spatial components of four vectors as three vectors.  To that end also write the components of the tensor $F_{\mu\nu}$ in terms of three vectors.
$$ F_{0i} = E^i , \; F_{ij} = -\epsilon_{ijk} B^k $$



Regular spatial vectors are ``naturally raised" while $D_i$ is ``naturally lowered".  Then we can rewrite \eqref{eq:s1:w0i}.
%TODO define D_i and \v{D}
\beq
	-im D_0 \eta_i =  - m^2 W_i  - \frac{i e \lambda}{m^2} \left( i e \lambda W^j E^j - D^j W_{j0} \right ) E^i
	+ ie \lambda W^j \epsilon_{ijk} B^k - D^j (  D_j W_i - D_i W_j )
\eeq

\beq
	i D_0 \eta^i =  m W^i  + \frac{i e \lambda}{m^3} \left( i e \lambda W^j E^j - D^j W_{j0} \right ) E^i
	- \frac{ie \lambda}{m} W^j \epsilon_{ijk} B^k + \frac{1}{m}D_j (  D_j W^i - D_i W^j )
\eeq

And likewise \eqref{eq:s1:wi} becomes
\beq
		D^0 W_i = D_i \frac{1}{m^2}\left( -i e \lambda W^j E^j - im  D^j \eta_j \right )  - im \eta_i
\eeq
\beq
		i D^0 W^i = - i D_i \frac{1}{m^2}\left( -i e \lambda W^j E^j - i m  D_j \eta^j \right )  + m \eta^i
\eeq

\beq
	i D^0 W^i= -\frac{1}{m^2} D_i  e \lambda \v{W} \cdot \v{E} - \frac{1}{m} D_i \v{D} \cdot \v{\eta} + m \eta^i
\eeq

\subsubsection{Spin identities}
To obtain some Schrodinger like equation for a bispinor, we need to express the time derivative of the bispinor in terms of other operators which can be interpreted as the Hamiltonian: $i \partial_0 \Psi = \hat{H} \Psi$.  We have expressions for the time derivatives of $W_i$ and $\eta_i$, but some mixing of the indices is involved.  To write the Hamiltonian in a block form we can introduce spin matrices whose action will mix the components of the fields.
	

The spin matrix for a spin one particle can represented as:
\beq
	(S^k)_{ij} = - i\epsilon_{ijk}
\eeq
which leads to the following identities:
\beq
	(\v{a} \times \v{v})_i = -i (\v{S} \cdot \v{a})_{ij} v_j
\eeq
\beq
	\{ \v{a} \times (\v{a} \times \v{v}) \}_i = - ( \{\v{S} \cdot \v{a}\}^2)_{ij} v_j
\eeq

\beq
	a_i (\v{b} \cdot \v{v}) = \{ \v{a} \cdot \v{b} \; \delta_{ij} - (S^k S^\ell)_{ij} a^\ell b^k \} v_j
\eeq

Using these identities

\beq
	i D^0 \v{W}= -\frac{e \lambda}{m^2} \v{D}   (\v{W} \cdot \v{E}) + \frac{1}{m} \v{D} (\v{D} \cdot \gv{\eta}) + m \gv{\eta}
\eeq

\beq
	i D^0 \v{W} = 
		-\frac{1}{m^2} \{ \v{D} \cdot \v{E} - (\v{S} \cdot \v{E}) (\v{S} \cdot \v{D})	\} \v{W}
		+ \frac{1}{m}\{ \v{D}^2 -  (\v{S} \cdot \v{D})^2 \} \gv{\eta} + m \gv{\eta}
\eeq
and for the other equation
\beq
	i D_0 \eta^i =  m W^i  - \frac{i e \lambda}{m^3} \left( i e \lambda W^j E^j - D^j W_{j0} \right ) E^i
	+ \frac{ie \lambda}{m} W^j \epsilon_{ijk} B^k - \frac{1}{m}D_j (  D_j W^i - D_i W^j )
\eeq

\beq
	i D_0 \eta^i =  m W^i  - \frac{i e \lambda}{m^3} \left( i e \lambda W^j E^j - D^j W_{j0} \right ) E^i
	+ \frac{ie \lambda}{m} W^j \epsilon_{ijk} B^k - \frac{1}{m}D_j (  D_j W^i - D_i W^j )
\eeq

\beq
	i D_0 \gv{\eta} = m \v{W} 
			+ \frac{e^2 \lambda^2}{m^3} \v{E} (\v{W} \cdot \v{E} )
			- \frac{1}{m^2} \v{E} (\v{D} \cdot \gv{\eta})
			+ \frac{i e \lambda}{m} (\v{W} \times \v{B} )
			+\frac{1}{m} \v{D} \times (\v{D} \times \v{W} ) 
\eeq

%TODO check order of D and E -- it matters!
\beq
	i D_0 \gv{\eta} = m \v{W} 
			+ \frac{e^2 \lambda^2}{m^3} \{ \v{E}^2 - (\v{S} \cdot \v{E})^2 \} \v{W}
			-\frac{1}{m^2} \{ \v{E} \cdot \v{D} - (\v{S} \cdot \v{E}) (\v{S} \cdot \v{D}) \} \gv{\eta}
			+ \frac{ e \lambda}{m} (\v{S} \cdot \v{B} ) \v{W}
			 - \frac{1}{m} (\v{S} \cdot \v{D})^2  \v{W}  
\eeq

\beq
	i D_0 \gv{\eta} = \left(
				m 
				+ \frac{e^2 \lambda^2}{m^3} \{ \v{E}^2 - (\v{S} \cdot \v{E})^2 \} 
				- \frac{ e \lambda}{m} (\v{S} \cdot \v{B} )
				- \frac{1}{m} (\v{S} \cdot \v{D})^2 
			\right ) \v{W} 
			+\frac{1}{m^2} \{ \v{E} \cdot \v{D} - (\v{S} \cdot \v{E}) (\v{S} \cdot \v{D}) \} \gv{\eta}  
\eeq

Now that the equations are in the correct form, we can write them as follows:



%%TODO This is the correct form, but go back and make sure equations leading up to this don't have sign errors
%% Also, add the spin ids that produce the cross products.
\beq
i D_0 \spinor{W}{\eta} = 
	\Mblock
	{ \lambda \frac{e}{m^2} \left [ \v{E} \cdot \v{D} - (\v{S} \cdot \v{E})( \v{S} \cdot \v{D}) + i \v{S} \cdot \v{E} \times \v{D} \right ] }
		{m
	-\frac{1}{m} (\v{S} \cdot \v{D})^2 
	- \lambda \frac{e}{m} \v{S} \cdot \v{B}
	+ \lambda^2 \frac{e^2}{m^3} \left [ \v{E}^2 - (\v{S} \cdot \v{E})^2 \right ]  }
	{ m
	- \frac{1}{m}\left [ \v{D}^2 - (\v{S} \cdot \v{D})^2 + e \v{S} \cdot \v{B} \right ]  }
	{ - \lambda \frac{e}{m^2} \left [ \v{D} \cdot \v{E} - (\v{S} \cdot \v{D}) (\v{S} \cdot \v{E}) + i \v{S} \cdot \v{D} \times \v{E} \right ]  }\eeq




\subsubsection{Current}

We can also derive the conserved current from the Lagrangian:
\begin{eqnarray*}
\mathcal{L} 
	&=&	-\frac{1}{2} (D \times W)^\dagger \cdot (D \times W) 
				+ m_w^2 W^\dagger W 
				-\lambda i e {W^\dagger}^\mu W^\nu F_{\mu \nu}	\\
\end{eqnarray*}

Where
\begin{eqnarray*}
		D^\mu	=	\partial^\mu - i e A^\mu ,
	&&
		D \times W = D^\mu W^\nu - D^\nu W^\mu
\end{eqnarray*}


We want the conserved current corresponding to the transformation $ W_i \to e^{i \alpha}W_i $, which in infinitesimal form is:
\begin{equation*}
	W_\mu \to W_\mu + i \alpha W_\mu, \;
	W_\mu^\dagger \to W_\mu^\dagger - i \alpha W_\mu^{\dagger}
\end{equation*}

The 4-current density will be:
\begin{equation*}
j^{\sigma} = -i \pd {\mathcal{L} }{W_{\mu, \sigma}} W_\mu  +  i\pd {\mathcal{L} }{W^\dagger_{\mu, \sigma}} W^\dagger_\mu
\end{equation*}

Only one term contains derivatives of the field:

\begin{eqnarray*}
 \pd {\mathcal{L} }{W_{\alpha, \sigma}} 
		&=& \pd{}{W_{\alpha, \sigma}} \left \{ - \frac{1}{2} (D_\mu W_\nu - D_\nu W_\mu)^\dagger(D^\mu W^\nu - D^\nu W^\mu) \right \}\\
		&=& - \frac{1}{2} (D_\mu W_\nu - D_\nu W_\mu)^\dagger (g_{\sigma \mu} g_{\alpha \nu} - g_{\sigma \nu}g_{\alpha \mu})\\
		&=& - (D_\alpha W_\sigma - D_\sigma W_\alpha)^\dagger
\end{eqnarray*}
Likewise:
\begin{eqnarray*}
	\pd {\mathcal{L} }{W_{\alpha, \sigma}^\dagger} 
		&=& - (D_\alpha W_\sigma - D_\sigma W_\alpha)
\end{eqnarray*}

If  we define $W_{\mu \nu} =  D^\mu W^\nu - D^\nu W^\mu$ then the 4-current and charge density are:

\begin{eqnarray*}
	j_\sigma &=& i W_{\sigma \mu}^\dagger W^{\mu} - i W_{\sigma \mu} {W^{\dagger}}^\mu \\
	j_0 	&=& i W_{0 \mu}^\dagger W^{\mu} - i W_{0 \mu} {W^{\dagger}}^\mu \\
		&=& i W_{0 i}^\dagger W^i - i W_{0 i} {W^{\dagger}}^i \\
\end{eqnarray*}
Where the last equality follows from the antisymmetry of $W_{\mu \nu}$.

Now, we defined the fields $\eta_i = -i \frac{W_{i0}}{m}$.  In terms of these fields,
$j_0 =  m (\eta_i^\dagger  W^i + \eta_i {W^\dagger}^i )$. 

We can do the same to find the vector part of the current.
\begin{eqnarray*}
	j_i &=& i W_{i \mu}^\dagger W^{\mu} - i W_{i \mu} {W^{\dagger}}^\mu 	\\
	&=&	i W_j^\dagger W_{ij}  + i W_{i0}^\dagger W_0 + c.c.
\end{eqnarray*}

We have $W_{ij} = D_i W_j - D_j W_i$.  Using the identities developed in the appendix, we can obtain
\[ D_j W_i = D_i W_j - D_k(S_i S_k)_{ja} W_a 	\]
Then
\[ W_{ij} = D_k (S_i S_k)_{ja} W_a 	\]

In the absence of an electric field E, $W_{0} = \frac{i}{m} D_j \eta_j$, with $W_{i0} = i m \eta_i$.
\[	W_{i0}^\dagger W_0 = - \eta_i^\dagger D_j \eta_j 	\]
Again we introduce spin matrices to get the equation in the desired form, and obtain
\[	W_{i0}^\dagger W_0 = - \eta_j^\dagger D_k (\delta_{ik} - S_k S_i) \eta_j 	\]

This leads to
\[ j_i = i W_j^\dagger D_k (S_i S_k W)_j - i \eta_j^\dagger D_k ([\delta_{ik} - S_k S_i]\eta)_j + c.c. \]

Writing this in terms of the bispinor $\begin{pmatrix}\eta \\ W\end{pmatrix}$, the expression for the current is

\begin{equation}	j_i	=
		\frac{i}{2} \begin{pmatrix}\eta^\dagger && W^\dagger \end{pmatrix} \left [
		(\{S_i, S_j\} - \delta_{ij})  
		\begin{pmatrix} 
			1 & 0 \\
			0 & 1 \\ 
		\end{pmatrix}
		- ([S_i, S_j] +\delta_{ij})	\begin{pmatrix} 1 & 0 \\ 0 & -1 \\ \end{pmatrix}
		\right ]
		D_j \begin{pmatrix}\eta \\ W\end{pmatrix} + c.c.
\end{equation}





